Remove Sawtooth from SimI.

theories/IL/BlockType.v
@@ -19,7 +19,6 @@ Instance block_type_F : BlockType (F.block) :=
     block_Z := F.block_Z
   }.
 
-
 Lemma mkBlocks_I_less
   : forall (F : list (params * stmt)) (n k : nat) (b : I.block),
     get (mapi_impl I.mkBlock k F) n b -> I.block_n b <= k + length F - 1.
@@ -33,7 +32,6 @@ Proof.
   intros; inv_get; eauto.
 Qed.
 
-
 Lemma mkBlocks_F_less
   : forall E (F : list (params * stmt)) (n k : nat) (b : F.block),
     get (mapi_impl (F.mkBlock E) k F) n b -> F.block_n b <= k + length F - 1.
@@ -45,4 +43,27 @@ Lemma mkBlock_F_i E F
   : forall i b, get (mapi (F.mkBlock E) F) i b -> i = F.block_n b.
 Proof.
   intros; inv_get; eauto.
+Qed.
+
+Definition smaller {B} `{BlockType B} (L:list B) :=
+        forall f b, get L f b -> f >= block_n b.
+
+Lemma smaller_I_mkBlocks L F
+  : smaller L
+    -> smaller (mapi I.mkBlock F ++ L).
+Proof.
+  intros; hnf; intros.
+  eapply get_app_cases in H0.
+  destruct H0; dcr; inv_get; simpl; eauto.
+  exploit H; eauto; simpl in *. omega.
+Qed.
+
+Lemma smaller_F_mkBlocks E L F
+  : smaller L
+    -> smaller (mapi (F.mkBlock E) F ++ L).
+Proof.
+  intros; hnf; intros.
+  eapply get_app_cases in H0.
+  destruct H0; dcr; inv_get; simpl; eauto.
+  exploit H; eauto; simpl in *. omega.
 Qed.
